experiment/Experiment.Steel.CondSolver.fsti
@@ -4,6 +4,7 @@ module M    = Experiment.Steel.Repr.M
 module U    = Learn.Util
 module L    = FStar.List.Pure
 module Ll   = Learn.List
+module SE   = Steel.Effect
 module Fin  = FStar.Fin
 module Opt  = Learn.Option
 module Perm = Learn.Permutation
@@ -202,6 +203,195 @@ let build_elem_index () : Tac unit =
   norm [delta_only [`%findi_true; `%Opt.map];
        iota; zeta; primops];
   cs_try trefl (fun m -> fail (m Fail_elem_index [Info_goal goal]))
+
+
+(*** Building a [M.to_repr_t] *)
+
+/// Steps for normalizing [M.flatten_vprop v].
+let __normal_flatten_vprop : list norm_step = [
+  delta_only [`%M.flatten_vprop; `%M.flatten_vprop_aux];
+  delta_attr [`%SE.__reduce__];
+  delta_qualifier ["unfold"];
+  iota; zeta; primops
+]
+
+/// Steps for the normalisation of Steel's requires and ensures clauses.
+/// We need [__steel_reduce__] in order to unfold the selector functions
+/// (for instance [Steel.Reference.sel])
+let __normal_Steel_logical_spec : list norm_step = [
+  delta_only [`%SE.VUnit?._0];
+  delta_attr [`%SE.__reduce__; `%SE.__steel_reduce__];
+  delta_qualifier ["unfold"];
+  iota; zeta; primops
+]
+
+
+val __build_to_repr_t_lem
+      (p : SE.vprop) (r_p : M.vprop_list {p `SE.equiv` M.vprop_of_list r_p}) (h : SE.rmem p)
+      (v : SE.vprop{SE.can_be_split p v}) (_ : squash (SE.VUnit? v))
+      (i : elem_index (SE.VUnit?._0 v) r_p)
+      (i' : int) (_ : squash (i' == i))
+  : squash (h v ==
+        M.sel r_p (SE.equiv_can_be_split p (M.vprop_of_list r_p);
+                   SE.focus_rmem h (M.vprop_of_list r_p)) i)
+
+[@@ __tac_helper__]
+let __build_to_repr_t
+      (#a : Type) (#pre : SE.pre_t) (#post : SE.post_t a) (#req : SE.req_t pre) (#ens : SE.ens_t pre a post)
+
+      (e_pre  : M.vprop_with_emp pre) (r_pre  : M.pre_t)
+      (pre_eq  : squash (r_pre == M.flatten_vprop e_pre))
+
+      (e_post : (x : a) -> M.vprop_with_emp (post x)) (r_post : M.post_t a)
+      (post_eq : (x : a) -> squash (r_post x == M.flatten_vprop (e_post x)))
+
+      (#r_req  : M.req_t r_pre)
+      (r_req_eq  : (h0 : SE.rmem pre) -> (sl0 : M.sl_f r_pre) ->
+                   (sl0_eq : ((v : SE.vprop{SE.can_be_split pre v}) -> squash (SE.VUnit? v) ->
+                             (i : elem_index (SE.VUnit?._0 v) r_pre) ->
+                             // This indirection is needed so that [apply_raw] presents a goal for [i]
+                             (i' : int) -> (_ : squash (i' == i)) ->
+                             squash (h0 v == sl0 i'))) ->
+                    r_req sl0 == req h0)
+
+      (#r_ens  : M.ens_t r_pre a r_post)
+      (r_ens_eq  : (h0 : SE.rmem pre) -> (sl0 : M.sl_f r_pre) ->
+                   (x : a) ->
+                   (h1 : SE.rmem (post x)) -> (sl1 : M.sl_f (r_post x)) ->
+                   (sl0_eq : ((v : SE.vprop{SE.can_be_split pre v}) -> squash (SE.VUnit? v) ->
+                             (i : elem_index (SE.VUnit?._0 v) r_pre) ->
+                             (i' : int) -> (_ : squash (i' == i)) ->
+                             squash (h0 v == sl0 i'))) ->
+                   (sl1_eq : ((v : SE.vprop{SE.can_be_split (post x) v}) -> squash (SE.VUnit? v) ->
+                             (i : elem_index (SE.VUnit?._0 v) (r_post x)) ->
+                             (i' : int) -> (_ : squash (i' == i)) ->
+                             squash (h1 v == sl1 i'))) ->
+                   r_ens sl0 x sl1 == ens h0 x h1)
+
+  : M.to_repr_t a pre post req ens
+  = 
+    let r_pre_eq () : Lemma (pre `SE.equiv` M.vprop_of_list r_pre)
+      = pre_eq;
+        M.vprop_equiv_flat pre e_pre;
+        SE.equiv_sym (M.vprop_of_list r_pre) pre                in
+    let r_post_eq (x : a) : Lemma (post x `SE.equiv` M.vprop_of_list (r_post x))
+      = post_eq x;
+        M.vprop_equiv_flat (post x) (e_post x);
+        SE.equiv_sym (M.vprop_of_list (r_post x)) (post x)
+    in
+    {
+    r_pre; r_post; r_req; r_ens;
+    r_pre_eq; r_post_eq;
+    r_req_eq  = (fun (h0 : SE.rmem pre) ->
+                   r_pre_eq ();
+                   SE.equiv_can_be_split pre (M.vprop_of_list r_pre);
+                   let h0_r = SE.focus_rmem h0 (M.vprop_of_list r_pre) in
+                   r_req_eq h0 (M.sel r_pre h0_r)
+                            (__build_to_repr_t_lem pre r_pre h0));
+    r_ens_eq  = (fun (h0 : SE.rmem pre) (x : a) (h1 : SE.rmem (post x)) ->
+                   r_pre_eq ();
+                   SE.equiv_can_be_split pre (M.vprop_of_list r_pre);
+                   let h0_r = SE.focus_rmem h0 (M.vprop_of_list r_pre) in
+                   r_post_eq x;
+                   SE.equiv_can_be_split (post x) (M.vprop_of_list (r_post x));
+                   let h1_r = SE.focus_rmem h1 (M.vprop_of_list (r_post x)) in
+                   r_ens_eq h0 (M.sel r_pre h0_r) x h1 (M.sel (r_post x) h1_r)
+                            (__build_to_repr_t_lem pre r_pre h0)
+                            (__build_to_repr_t_lem (post x) (r_post x) h1))
+  }
+
+let filter_rmem_apply (#p : SE.vprop) (h : SE.rmem p) (v : SE.vprop{SE.can_be_split p v})
+  #sl (_ : squash (h v == sl))
+  : squash (h v == sl)
+  = ()
+
+/// Given a term [squash (lhs == rhs)], this tactics returns [Some (h, v)] if [lhs] is [h v]
+/// UNUSED: using v generates a SMT goal [SE.can_be_split]
+let match_rmem_apply (t : term) : Tac (option (term & term))
+  = match inspect t with
+    | Tv_App _squash (eq, Q_Explicit) ->
+      let _, ts = collect_app eq in
+      let n_args = L.length ts in
+      if n_args <> 3 then fail ("unexpected shape1:"^string_of_int n_args)
+      else let lhs = (L.index ts 1)._1 in
+     (match inspect lhs with
+      | Tv_App h (v, Q_Explicit) -> Some (h, v)
+      | _ -> None)
+    | _ -> fail "unexpected shape0"
+
+#push-options "--ifuel 2"
+(**) private val __begin_opt_1 : unit
+
+/// Solves a goal [to_repr_t a pre post req ens]
+let build_to_repr_t () : Tac unit
+  =
+    let u_r_pre  = fresh_uvar None in
+    let u_r_post = fresh_uvar None in
+    let u_r_req  = fresh_uvar None in
+    let u_r_ens  = fresh_uvar None in
+    apply_raw (`__build_to_repr_t);
+
+    (* [r_pre] *)
+    build_vprop_with_emp ();
+    exact u_r_pre;
+    norm __normal_flatten_vprop;
+    trefl ();
+
+    (* [r_post] *)
+    let _ = intro () in
+      build_vprop_with_emp ();
+    exact u_r_post;
+    let _ = intro () in
+      norm __normal_flatten_vprop;
+      trefl ();
+
+    // apply the rewriting hypothesis [eq_lem] to solve a goal [squash (h v == sl ?i)]
+    let apply_rew eq_lem =
+      apply_raw eq_lem;
+      // [VUnit?]
+      norm [delta_only [`%SE.VUnit?]; iota];
+      trivial ();
+      // [elem_index]
+      norm __normal_Steel_logical_spec;
+      build_elem_index ();
+      // [i' <- i]
+      norm [delta_attr [`%__cond_solver__; `%__tac_helper__]];
+      trefl ()
+    in
+
+    (* [r_req] *)
+    exact u_r_req;
+    let h0 = intro () in let sl0 = intro () in let eq0 = intro () in
+      // This normalisation has to be done after introducing [eq0], otherwise its application fails,
+      // seemingly because of the normalisation of [t_of].
+      norm __normal_Steel_logical_spec;
+      pointwise begin fun () ->
+        match catch (fun () -> apply_raw (`filter_rmem_apply (`#h0))) with
+        | Inr () -> // For some reason, this can only be applied on the goal produced by [filter_rmem_apply]
+                   apply_rew eq0
+        | Inl _  -> trefl ()
+      end;
+      trefl ();
+
+    (* [r_ens] *)
+    exact u_r_ens;
+    let h0  = intro () in let sl0 = intro () in
+    let x   = intro () in
+    let h1  = intro () in let sl1 = intro () in
+    let eq0 = intro () in let eq1 = intro () in
+      norm __normal_Steel_logical_spec;
+      pointwise begin fun () ->
+        match catch (fun () -> apply_raw (`filter_rmem_apply (`#h0))) with
+        | Inr () -> apply_rew eq0
+        | Inl _ ->
+        match catch (fun () -> apply_raw (`filter_rmem_apply (`#h1))) with
+        | Inr () -> apply_rew eq1
+        | Inl _  -> trefl ()
+      end;
+      trefl ()
+
+#pop-options
+(**) private val __end_opt_1 : unit
 
 
 (*** Building an injection *)
@@ -687,9 +877,13 @@ let __build_TCspec_u
   : M.tree_cond (M.Tspec a pre post req ens) pre' (fun (x : a) -> L.(post x @ cond_sol_unmatched_v cs0))
   =
     let frame = cond_sol_unmatched_v cs0 in
-    M.TCspec pre' (fun x -> L.(post x @ frame)) frame
-             (serialize_perm (cond_sol_to_equiv cs0))
-             (fun x -> Perm.id_n (len L.(post x @ frame)))
+    M.TCspec M.({
+      tcs_pre     = pre';
+      tcs_post    = (fun x -> L.(post x @ frame));
+      tcs_frame   = frame;
+      tcs_pre_eq  = serialize_perm (cond_sol_to_equiv cs0);
+      tcs_post_eq = (fun x -> Perm.id_n (len L.(post x @ frame)))
+    })
 
 [@@ __tac_helper__]
 let __build_TCspec_p
@@ -706,9 +900,62 @@ let __build_TCspec_p
 
   : M.tree_cond (M.Tspec a pre post req ens) pre' post'
   =
-    M.TCspec pre' post' (cond_sol_unmatched_v cs0)
-             (serialize_perm (cond_sol_to_equiv cs0))
-             (fun x -> serialize_perm (cond_sol_all_to_equiv (cs1 x)))
+    M.TCspec M.({
+      tcs_pre     = pre';
+      tcs_post    = post';
+      tcs_frame   = cond_sol_unmatched_v cs0;
+      tcs_pre_eq  = serialize_perm (cond_sol_to_equiv cs0);
+      tcs_post_eq = (fun x -> serialize_perm (cond_sol_all_to_equiv (cs1 x)))
+    })
+
+// TODO? currently, one cannot factorize the tree_cond_spec part of TCspec & TCspecS
+// since there are constraints on tcs_pre & tcs_post
+[@@ __tac_helper__]
+let __build_TCspecS_u
+      (#a : Type) (#pre : SE.pre_t) (#post : SE.post_t a) (#req : SE.req_t pre) (#ens : SE.ens_t pre a post)
+      (#pre' : M.pre_t)
+      (tr  : M.to_repr_t a pre post req ens)
+      (cs0 : cond_sol false tr.r_pre pre')
+
+      (pre_n   : extract_term (L.length tr.r_pre))
+      (post_n  : (x : a) -> extract_term (L.length (tr.r_post x)))
+      (frame_n : extract_term (L.length (cond_sol_unmatched cs0)))
+      (p0 : __extract_perm (cond_sol_to_equiv cs0))
+
+  : M.tree_cond (M.TspecS a pre post req ens) pre' (fun (x : a) -> L.(tr.r_post x @ cond_sol_unmatched_v cs0))
+  =
+    let frame = cond_sol_unmatched_v cs0 in
+    M.TCspecS tr M.({
+      tcs_pre     = pre';
+      tcs_post    = (fun x -> L.(tr.r_post x @ frame));
+      tcs_frame   = frame;
+      tcs_pre_eq  = serialize_perm (cond_sol_to_equiv cs0);
+      tcs_post_eq = (fun x -> Perm.id_n (len L.(tr.r_post x @ frame)))
+    })
+
+[@@ __tac_helper__]
+let __build_TCspecS_p
+      (#a : Type) (#pre : SE.pre_t) (#post : SE.post_t a) (#req : SE.req_t pre) (#ens : SE.ens_t pre a post)
+      (#pre' : M.pre_t) (#post' : M.post_t a)
+      (tr  : M.to_repr_t a pre post req ens)
+      (cs0 : cond_sol false tr.r_pre pre')
+      (cs1 : (x : a) -> cond_sol true (post' x) L.(tr.r_post x @ cond_sol_unmatched_v cs0))
+
+      (pre_n   : extract_term (L.length tr.r_pre))
+      (post_n  : (x : a) -> extract_term (L.length (tr.r_post x)))
+      (frame_n : extract_term (L.length (cond_sol_unmatched cs0)))
+      (p0 : __extract_perm (cond_sol_to_equiv cs0))
+      (p1 : (x : a) -> __extract_perm (cond_sol_all_to_equiv (cs1 x)))
+
+  : M.tree_cond (M.TspecS a pre post req ens) pre' post'
+  =
+    M.TCspecS tr M.({
+      tcs_pre     = pre';
+      tcs_post    = post';
+      tcs_frame   = cond_sol_unmatched_v cs0;
+      tcs_pre_eq  = serialize_perm (cond_sol_to_equiv cs0);
+      tcs_post_eq = (fun x -> serialize_perm (cond_sol_all_to_equiv (cs1 x)))
+    })
 
 
 /// By default, if the post-condition of a [M.Tret] has to be inferred, we simply choose [fun _ -> pre]. That is,
@@ -747,9 +994,15 @@ let __build_TCret_p
     M.TCret #a #x pre post (serialize_perm (cond_sol_all_to_equiv cs))
 
 
-let build_TCspec (post : bool) : Tac shape_tree_t
-  = if post then begin
-      apply_raw (`__build_TCspec_p);
+let build_TCspec (is_Steel : bool) (post : bool) : Tac shape_tree_t
+  =
+    if post then begin
+      if is_Steel then (
+        apply_raw (`__build_TCspecS_p);
+        build_to_repr_t ();
+        norm_cond_sol ()
+      ) else
+        apply_raw (`__build_TCspec_p);
       build_cond_sol false;
       norm_cond_sol ();
       let x = intro () in
@@ -757,8 +1010,17 @@ let build_TCspec (post : bool) : Tac shape_tree_t
     end else begin
       // FIXME : why apply_raw shelves cs0 ?
       let cs0 = fresh_uvar None in
-      apply_raw (`(__build_TCspec_u (`#cs0)));
-      unshelve cs0;
+      if is_Steel then (
+        let tr = fresh_uvar None in
+        apply_raw (`(__build_TCspecS_u (`#tr) (`#cs0)));
+        unshelve tr;
+        build_to_repr_t ();
+        unshelve cs0;
+        norm_cond_sol ()
+      ) else (
+        apply_raw (`(__build_TCspec_u (`#cs0)));
+        unshelve cs0
+      );
       build_cond_sol false
     end;
 
@@ -817,7 +1079,8 @@ and build_tree_cond (post : bool) : Tac shape_tree_t
           let nd = inspect_fv fv in
           if Nil? nd then (let _ = fail_shape () in fail "unreachable");
           begin match L.last nd with
-          | "Tspec"  -> build_TCspec
+          | "Tspec"  -> build_TCspec false
+          | "TspecS" -> build_TCspec true
           | "Tret"   -> build_TCret 
           | "Tbind"  -> build_TCbind
           | "TbindP" -> build_TCbindP
@@ -900,5 +1163,6 @@ let build_prog_cond () : Tac unit
                       `%L.length; `%L.hd; `%L.tl; `%L.tail; `%L.index; `%Ll.initi; `%Ll.list_eq;
                       `%U.cast];
           delta_qualifier ["unfold"];
+          delta_attr [`%__tac_helper__];
           iota; zeta; primops; simplify];
     exact (`intro_l_True)
