experiment/Experiment.Steel.Repr.M.fsti
@@ -10,9 +10,6 @@ module Mem  = Steel.Memory
 module Perm = Learn.Permutation
 module FExt = FStar.FunctionalExtensionality
 
-open FStar.Calc
-open FStar.Classical.Sugar
-
 open Steel.Effect
 open Steel.Effect.Atomic
 
@@ -50,6 +47,23 @@ let subcomp_no_frame_pre
         ens_f (focus_rmem h0 pre_f) x (focus_rmem h1 (post_f x)) ==>
         ens_g h0 x h1))))))
 
+val intro_subcomp_no_frame_pre
+      (#a:Type)
+      (#pre_f:pre_t) (#post_f:post_t a) (req_f:req_t pre_f) (ens_f:ens_t pre_f a post_f)
+      (#pre_g:pre_t) (#post_g:post_t a) (req_g:req_t pre_g) (ens_g:ens_t pre_g a post_g)
+      (eq_pre  : squash (equiv pre_g pre_f))
+      (eq_post : (x : a) -> squash (equiv (post_g x) (post_f x)))
+      (s_pre :  (h0 : rmem pre_g) -> Lemma
+         (requires can_be_split pre_g pre_f /\
+                   req_g h0)
+         (ensures  req_f (focus_rmem h0 pre_f)))
+      (s_post : (h0 : rmem pre_g) -> (x : a) -> (h1 : rmem (post_g x)) -> Lemma
+         (requires can_be_split pre_g pre_f /\ can_be_split (post_g x) (post_f x) /\
+                   req_g h0 /\ req_f (focus_rmem h0 pre_f) /\
+                   ens_f (focus_rmem h0 pre_f) x (focus_rmem h1 (post_f x)))
+         (ensures  ens_g h0 x h1))
+  : squash (subcomp_no_frame_pre req_f ens_f req_g ens_g eq_pre eq_post)
+
 inline_for_extraction noextract
 val unit_steel_subcomp_no_frame
       (#a : Type)
@@ -58,7 +72,7 @@ val unit_steel_subcomp_no_frame
       (eq_pre  : squash (equiv pre_g pre_f))
       (eq_post : (x : a) -> squash (equiv (post_g x) (post_f x)))
       (sb_pre : squash (subcomp_no_frame_pre req_f ens_f req_g ens_g eq_pre eq_post))
-      (f : unit_steel a pre_f post_f req_f ens_f)
+      ($f : unit_steel a pre_f post_f req_f ens_f)
   : unit_steel a pre_g post_g req_g ens_g
 
 
@@ -255,7 +269,8 @@ val steel_change_vequiv (#vs0 #vs1 : vprop_list) (#opened:Mem.inames) (f : vequi
       (requires fun _ -> True)
       (ensures fun h0 () h1 -> sel_f vs1 h1 == extract_vars f (sel_f vs0 h0))
 
-(*** [prog_tree] *)
+
+(*** [repr_steel_t] *)
 
 type pre_t = vprop_list
 type post_t (a : Type) = a -> vprop_list
@@ -263,22 +278,111 @@ type post_t (a : Type) = a -> vprop_list
 type req_t (pre : pre_t) = sl_f pre -> Type0
 type ens_t (pre : pre_t) (a : Type) (post : post_t a) = sl_f pre -> (x : a) -> sl_f (post x) -> Type0
 
+type repr_steel_t (a : Type)
+       (pre : pre_t) (post : post_t a)
+       (req : req_t pre) (ens : ens_t pre a post) : Type
+  = unit_steel a
+      (vprop_of_list pre) (fun x -> vprop_of_list (post x))
+      (requires fun h0      -> req (sel pre h0))
+      (ensures  fun h0 x h1 -> ens (sel pre h0) x (sel_f (post x) h1))
+
+inline_for_extraction noextract
+let repr_steel_subcomp
+      (#a : Type) (#pre : pre_t) (#post : post_t a)
+      (req_f : req_t pre) (ens_f : ens_t pre a post)
+      (req_g : req_t pre) (ens_g : ens_t pre a post)
+      (pf_req : (sl0 : sl_f pre) ->
+                Lemma (requires req_g sl0) (ensures req_f sl0))
+      (pf_ens : (sl0 : sl_f pre) -> (x : a) -> (sl1 : sl_f (post x)) ->
+                Lemma (requires req_f sl0 /\ req_g sl0 /\ ens_f sl0 x sl1) (ensures ens_g sl0 x sl1))
+      (r : repr_steel_t a pre post req_f ens_f)
+  : repr_steel_t a pre post req_g ens_g
+  = 
+    (fun () ->
+      (**) let sl0 : Ghost.erased (t_of (vprop_of_list pre)) = gget (vprop_of_list pre) in
+      (**) pf_req (vpl_sels_f pre sl0);
+      let x = r () in
+      (**) let sl1 : Ghost.erased (t_of (vprop_of_list (post x))) = gget (vprop_of_list (post x)) in
+      (**) pf_ens (vpl_sels_f pre sl0) x (vpl_sels_f (post x) sl1);
+      Steel.Effect.Atomic.return x)
+
+(*// This fail, seemingly because of the expansion of the memories when checking the post
+[@@ handle_smt_goals ]
+let tac () = dump "SMT query"
+let steel_of_repr
+      (#a : Type) (#pre : pre_t) (#post : post_t a) (#req : req_t pre) (#ens : ens_t pre a post)
+      (f : unit_steel a pre post req ens)
+  : Steel a pre post req ens
+  = f ()*)
+
+[@@ Learn.Tactics.Util.__tac_helper__]
+noeq
+type to_repr_t (a : Type) (pre : SE.pre_t) (post : SE.post_t a) (req : SE.req_t pre) (ens : SE.ens_t pre a post)
+= {
+  r_pre  : pre_t;
+  r_post : post_t a;
+  r_req  : req_t r_pre;
+  r_ens  : ens_t r_pre a r_post;
+  r_pre_eq  : unit -> Lemma (pre `equiv` vprop_of_list r_pre);
+  r_post_eq : (x : a) -> Lemma (post x `equiv` vprop_of_list (r_post x));
+  r_req_eq  : (h0 : rmem pre) -> Lemma (req h0 ==
+                  r_req (sel r_pre (
+                          r_pre_eq ();
+                          equiv_can_be_split pre (vprop_of_list r_pre);
+                          focus_rmem h0 (vprop_of_list r_pre))));
+  r_ens_eq  : (h0 : rmem pre) -> (x : a) -> (h1 : rmem (post x)) -> Lemma (ens h0 x h1 ==
+                  r_ens (sel r_pre (
+                          r_pre_eq ();
+                          equiv_can_be_split pre (vprop_of_list r_pre);
+                          focus_rmem h0 (vprop_of_list r_pre)))
+                        x
+                        (sel (r_post x) (
+                          r_post_eq x;
+                          equiv_can_be_split (post x) (vprop_of_list (r_post x));
+                          focus_rmem h1 (vprop_of_list (r_post x)))))
+}
+
+inline_for_extraction noextract
+val steel_of_repr
+      (#a : Type) (#pre : SE.pre_t) (#post : SE.post_t a) (#req : SE.req_t pre) (#ens : SE.ens_t pre a post)
+      (tr : to_repr_t a pre post req ens)
+      (f : repr_steel_t a tr.r_pre tr.r_post tr.r_req tr.r_ens)
+  : unit_steel a pre post req ens
+
+inline_for_extraction noextract
+val repr_steel_of_steel
+      (#a : Type) (#pre : SE.pre_t) (#post : SE.post_t a) (#req : SE.req_t pre) (#ens : SE.ens_t pre a post)
+      (tr : to_repr_t a pre post req ens)
+      ($f  : unit_steel a pre post req ens)
+  : repr_steel_t a tr.r_pre tr.r_post tr.r_req tr.r_ens 
+
+
+(*** [prog_tree] *)
+
 noeq
 type prog_tree : (a : Type u#a) -> Type u#(max (a+1) 2) =
+  // A specification of the subprogram, used to represent function calls
   | Tspec  : (a : Type u#a) -> (pre : pre_t) -> (post : post_t a) ->
              (req : req_t pre) -> (ens : ens_t pre a post) ->
              prog_tree a
+  // A Steel specification, used to represent calls to Steel functions
+  | TspecS : (a : Type u#a) -> (pre : SE.pre_t) -> (post : SE.post_t a) ->
+             (req : SE.req_t pre) -> (ens : SE.ens_t pre a post) ->
+             prog_tree a
+  // return, with a hint for introducing dependencies in the returned value
   | Tret   : (a : Type u#a) -> (x : a) -> (sl_hint : post_t a) ->
              prog_tree a
+  // bind
   | Tbind  : (a : Type u#a) -> (b : Type u#a) ->
              (f : prog_tree a) -> (g : a -> prog_tree b) ->
              prog_tree b
+  // bind pure, models a polymonadic bind between PURE and our monad
   | TbindP : (a : Type u#a) -> (b : Type u#a) ->
              (wp : pure_wp a) -> (x : unit -> PURE a wp) -> (g : a -> prog_tree b) ->
              prog_tree b
 
 
-(**** slprop unification conditions *)
+(*** slprop unification conditions *)
 
 (* TODO:
    - ? equalities vs vequiv
@@ -286,13 +390,27 @@ type prog_tree : (a : Type u#a) -> Type u#(max (a+1) 2) =
    - ~pr ! allow assumptions -> VC
    - ALT: recursively defined type *)
 
+[@@ Learn.Tactics.Util.__tac_helper__]
+noeq
+type tree_cond_Spec (a : Type) (pre : pre_t) (post : post_t a) = {
+  tcs_pre     : pre_t;
+  tcs_post    : post_t a;
+  tcs_frame   : vprop_list;
+  tcs_pre_eq  : vequiv tcs_pre L.(pre @ tcs_frame);
+  tcs_post_eq : (x : a) -> vequiv L.(post x @ tcs_frame) (tcs_post x)
+}
+
 noeq
 type tree_cond : (#a : Type u#a) -> (t : prog_tree a) -> (pre : pre_t) -> (post : post_t a) -> Type u#(max (a+1) 2) =
-  | TCspec  : (#a : Type u#a) -> (#pre : pre_t) -> (#post : post_t a) -> (#req : req_t pre) -> (#ens : ens_t pre a post) ->
-              (pre' : pre_t) -> (post' : post_t a) -> (frame : vprop_list) ->
-              (p0 : vequiv pre' L.(pre @ frame)) ->
-              (p1 : ((x : a) -> vequiv (post x @ frame) (post' x))) ->
-              tree_cond (Tspec a pre post req ens) pre' post'
+  | TCspec  : (#a : Type u#a) -> (#pre : pre_t) -> (#post : post_t a) ->
+              (#req : req_t pre) -> (#ens : ens_t pre a post) ->
+              (tcs : tree_cond_Spec a pre post) ->
+              tree_cond (Tspec a pre post req ens) tcs.tcs_pre tcs.tcs_post
+  | TCspecS : (#a : Type u#a) -> (#pre : SE.pre_t) -> (#post : SE.post_t a) ->
+              (#req : SE.req_t pre) -> (#ens : SE.ens_t pre a post) ->
+              (tr  : to_repr_t a pre post req ens) ->
+              (tcs : tree_cond_Spec a tr.r_pre tr.r_post) ->
+              tree_cond (TspecS a pre post req ens) tcs.tcs_pre tcs.tcs_post
   | TCret   : (#a : Type u#a) -> (#x : a) -> (#sl_hint : post_t a) ->
               (pre : pre_t) -> (post : post_t a) ->
               (p : vequiv pre (post x)) ->
@@ -323,47 +441,58 @@ type shape_tree : (pre_n : nat) -> (post_n : nat) -> Type =
              (g : shape_tree pre_n post_n) ->
              shape_tree pre_n post_n
 
-let rec tree_cond_has_shape (#a : Type) (#pre : pre_t) (#post0 : post_t a) (#t : prog_tree a)
-                            (c : tree_cond t pre post0)
-                            (#post_n : nat) (s : shape_tree (L.length pre) post_n)
+unfold
+let tree_cond_has_shape_Spec
+      (a : Type) (pre : pre_t) (post : post_t a) (tcs : tree_cond_Spec a pre post)
+      (#post_n : nat) (s : shape_tree (L.length tcs.tcs_pre) post_n)
+  : prop
+  = match s with
+  | Sspec pre_n post_n frame_n p0' p1' ->
+    pre_n = L.length pre /\
+    frame_n = L.length tcs.tcs_frame /\
+    Ll.list_eq
+      (Perm.perm_f_to_list
+        (U.cast #(Perm.perm_f L.(length tcs.tcs_pre)) (Perm.perm_f (pre_n + frame_n))
+          tcs.tcs_pre_eq))
+      p0' /\
+   (forall (x : a) .
+     L.length (post  x) = post_n /\
+     L.length (tcs.tcs_post x) = post_n + frame_n /\ (* already implied ? *)
+     Ll.list_eq
+       (Perm.perm_f_to_list
+         (U.cast #(Perm.perm_f L.(length (post x @ tcs.tcs_frame)))
+                  (Perm.perm_f (post_n + frame_n))
+                  (tcs.tcs_post_eq x)))
+       p1')
+  | _ -> False
+
+let rec tree_cond_has_shape
+      (#a : Type) (#pre : pre_t) (#post0 : post_t a) (#t : prog_tree a)
+      (c : tree_cond t pre post0)
+      (#post_n : nat) (s : shape_tree (L.length pre) post_n)
   : Pure prop (requires True) (ensures fun p -> p ==> (forall (x : a) . L.length (post0 x) = post_n)) (decreases c)
   = match c with
-  | TCspec #a #pre #post pre1 post1 frame p0 p1 ->
-                                  (match s with
-                                    | Sspec pre_n post_n frame_n p0' p1' ->
-                                      pre_n = L.length pre /\
-                                      frame_n = L.length frame /\
-                                      Ll.list_eq
-                                        (Perm.perm_f_to_list
-                                          (U.cast #(Perm.perm_f L.(length pre1)) (Perm.perm_f (pre_n + frame_n))
-                                            p0))
-                                        p0' /\
-                                     (forall (x : a) .
-                                       L.length (post  x) = post_n /\
-                                       L.length (post1 x) = post_n + frame_n /\ (* already implied ? *)
-                                       Ll.list_eq
-                                         (Perm.perm_f_to_list
-                                           (U.cast #(Perm.perm_f L.(length (post x @ frame)))
-                                                    (Perm.perm_f (post_n + frame_n))
-                                                    (p1 x)))
-                                         p1')
-                                    | _ -> False)
-  | TCret #a pre post p           -> (match s with
-                                    | Sret n p' ->
-                                      Ll.list_eq (Perm.perm_f_to_list #n p) p' /\
-                                     (forall (x : a) . L.length (post x) = n)
-                                    | _ -> False)
-  | TCbind #a #b pre itm post f g -> (match s with
-                                    | Sbind _ itm_n post_n s_f s_g ->
-                                      tree_cond_has_shape f s_f /\
-                                     (forall (x : a) . tree_cond_has_shape (g x) s_g) /\
-                                     (forall (y : b) . L.length (post y) = post_n)
-                                    | _ -> False)
-  | TCbindP #a #b pre post g      -> (match s with
-                                    | SbindP _ post_n s_g ->
-                                      (forall (x : a) . tree_cond_has_shape (g x) s_g) /\
-                                      (forall (y : b) . L.length (post y) = post_n)
-                                    | _ -> False)
+  | TCspec #a #pre #post tcs -> tree_cond_has_shape_Spec a pre post tcs s
+  | TCspecS #a tr tcs -> tree_cond_has_shape_Spec a tr.r_pre tr.r_post tcs s
+  | TCret #a pre post p ->
+      (match s with
+      | Sret n p' ->
+        Ll.list_eq (Perm.perm_f_to_list #n p) p' /\
+       (forall (x : a) . L.length (post x) = n)
+      | _ -> False)
+  | TCbind #a #b pre itm post f g ->
+      (match s with
+      | Sbind _ itm_n post_n s_f s_g ->
+        tree_cond_has_shape f s_f /\
+       (forall (x : a) . tree_cond_has_shape (g x) s_g) /\
+       (forall (y : b) . L.length (post y) = post_n)
+      | _ -> False)
+  | TCbindP #a #b pre post g ->
+      (match s with
+      | SbindP _ post_n s_g ->
+        (forall (x : a) . tree_cond_has_shape (g x) s_g) /\
+        (forall (y : b) . L.length (post y) = post_n)
+      | _ -> False)
 
 noeq inline_for_extraction
 type prog_cond (#a : Type) (t : prog_tree a) (pre : pre_t) (post : post_t a) = {
@@ -375,20 +504,34 @@ type prog_cond (#a : Type) (t : prog_tree a) (pre : pre_t) (post : post_t a) = {
 
 (**** requires / ensures *)
 
+(** spec *)
+
+let spec_req (#a : Type) (#pre : pre_t) (#post : post_t a) (tcs : tree_cond_Spec a pre post)
+             (req : req_t pre)
+  : req_t tcs.tcs_pre
+  = fun sl0 ->
+      req (extract_vars_f tcs.tcs_pre pre tcs.tcs_frame tcs.tcs_pre_eq sl0)._1
+
+let spec_ens (#a : Type) (#pre : pre_t) (#post : post_t a) (tcs : tree_cond_Spec a pre post)
+             (ens : ens_t pre a post)
+  : ens_t tcs.tcs_pre a tcs.tcs_post
+  = fun sl0' x sl1' ->
+      let sl0, frame0 = extract_vars_f tcs.tcs_pre pre tcs.tcs_frame tcs.tcs_pre_eq sl0' in
+      let sl1, frame1 = extract_vars_f (tcs.tcs_post x) (post x) tcs.tcs_frame
+                                       (Perm.pequiv_sym (tcs.tcs_post_eq x)) sl1' in
+      frame1 == frame0 /\ ens sl0 x sl1
+
 (** return *)
 
-unfold
 let return_req (pre : pre_t) : req_t pre
   = fun _ -> True
 
-unfold
 let return_ens (#a : Type) (x : a) (p : post_t a) : ens_t (p x) a p
   = fun sl0 r sl1 ->
       r == x /\ sl1 == sl0
 
 (** bind *)
 
-unfold
 let bind_req (#a : Type)
       (#pre : pre_t) (#itm : post_t a)
       (req_f : req_t pre) (ens_f : ens_t pre a itm)
@@ -401,7 +544,6 @@ let bind_req (#a : Type)
 /// Unlike the bind combiner of Steel, our ensures clause does not recall the pre-condition of [f] for
 /// the reason explained on [Experiment.Repr.Fun.tree_ens]
 
-unfold
 let bind_ens (#a : Type) (#b : Type)
       (#pre : pre_t) (#itm : post_t a) (#post : post_t b)
       (ens_f : ens_t pre a itm) (ens_g : (x:a) -> ens_t (itm x) b post)
@@ -413,14 +555,12 @@ let bind_ens (#a : Type) (#b : Type)
 
 (** bind_pure *)
 
-unfold
 let bind_pure_req (#a : Type) (wp : pure_wp a)
       (#pre : pre_t)
       (req : a -> req_t pre)
   : req_t pre
   = fun sl0 -> wp (fun x -> req x sl0)
 
-unfold
 let bind_pure_ens (#a : Type) (#b : Type)
       (wp : pure_wp a)
       (#pre : pre_t) (#post : post_t b)
@@ -435,8 +575,10 @@ let rec tree_req (#a : Type u#a) (t : prog_tree a)
                  (#pre : pre_t) (#post : post_t a) (c : tree_cond t pre post)
   : Tot (req_t pre) (decreases t) =
   match c with
-  | TCspec #_ #pre #_ #req #_  pre' _ frame  p0 _ ->
-             (fun sl0 -> req (extract_vars_f pre' pre frame p0 sl0)._1)
+  | TCspec #_ #pre #_ #req #_  tcs ->
+             spec_req tcs req
+  | TCspecS #_ tr tcs ->
+             spec_req tcs tr.r_req
   | TCret #_ #_  pre _  _ ->
              return_req pre
   | TCbind #_ #_ #f #g  pre itm _  cf cg ->
@@ -448,12 +590,10 @@ and tree_ens (#a : Type u#a) (t : prog_tree a)
              (#pre : pre_t) (#post : post_t a) (c : tree_cond t pre post)
   : Tot (ens_t pre a post) (decreases t) =
   match c with
-  | TCspec #a #pre #post #req #ens  pre' post' frame  p0 p1 ->
-             (fun sl0' x sl1' ->
-                let sl0, frame0 = extract_vars_f pre' pre frame p0 sl0' in
-                let sl1, frame1 = extract_vars_f (post' x) (post x) frame
-                                                 (Perm.pequiv_sym (p1 x)) sl1' in
-                frame1 == frame0 /\ ens sl0 x sl1)
+  | TCspec #a #pre #post #req #ens  tcs ->
+             spec_ens tcs ens
+  | TCspecS #_ tr tcs ->
+             spec_ens tcs tr.r_ens
   | TCret #a #x  pre post  p ->
              (fun sl0 x' sl1 ->
                 x' == x /\
@@ -467,35 +607,6 @@ and tree_ens (#a : Type u#a) (t : prog_tree a)
 
 (*** "Monad" *)
 
-type repr_steel_t (a : Type)
-       (pre : pre_t) (post : post_t a)
-       (req : req_t pre) (ens : ens_t pre a post) : Type
-  = unit_steel a
-      (vprop_of_list pre) (fun x -> vprop_of_list (post x))
-      (requires fun h0      -> req (sel pre h0))
-      (ensures  fun h0 x h1 -> ens (sel pre h0) x (sel_f (post x) h1))
-
-inline_for_extraction noextract
-let repr_steel_subcomp
-      (#a : Type) (#pre : pre_t) (#post : post_t a)
-      (req_f : req_t pre) (ens_f : ens_t pre a post)
-      (req_g : req_t pre) (ens_g : ens_t pre a post)
-      (pf_req : (sl0 : sl_f pre) ->
-                Lemma (requires req_g sl0) (ensures req_f sl0))
-      (pf_ens : (sl0 : sl_f pre) -> (x : a) -> (sl1 : sl_f (post x)) ->
-                Lemma (requires req_f sl0 /\ req_g sl0 /\ ens_f sl0 x sl1) (ensures ens_g sl0 x sl1))
-      (r : repr_steel_t a pre post req_f ens_f)
-  : repr_steel_t a pre post req_g ens_g
-  = 
-    (fun () ->
-      (**) let sl0 : Ghost.erased (t_of (vprop_of_list pre)) = gget (vprop_of_list pre) in
-      (**) pf_req (vpl_sels_f pre sl0);
-      let x = r () in
-      (**) let sl1 : Ghost.erased (t_of (vprop_of_list (post x))) = gget (vprop_of_list (post x)) in
-      (**) pf_ens (vpl_sels_f pre sl0) x (vpl_sels_f (post x) sl1);
-      Steel.Effect.Atomic.return x)
-
-
 /// We define a "monad" (which does not satisfy the monad laws) on a [repr] type which contains a representation
 /// of the program as a tree and a corresponding steel function.
 
@@ -506,44 +617,67 @@ type repr (a : Type) = {
                repr_steel_t a pre post (tree_req repr_tree c) (tree_ens repr_tree c)
 }
 
-[@@ __repr_M__]
-let tree_of_steel (#a : Type) (#pre : pre_t) (#post : post_t a) (#req : req_t pre) (#ens : ens_t pre a post)
-                  ($f : repr_steel_t a pre post req ens)
-  : prog_tree a
-  = Tspec a pre post req ens
-
 inline_for_extraction noextract
 let repr_of_steel_steel
       (a : Type) (pre : pre_t) (post : post_t a) (req : req_t pre) (ens : ens_t pre a post)
-      (pre' : pre_t) (post' : post_t a) (frame : vprop_list)
-      (p0 : vequiv pre' L.(pre @ frame)) (p1 : ((x : a) -> vequiv (post x @ frame) (post' x)))
+      (tcs : tree_cond_Spec a pre post)
       ($f : repr_steel_t a pre post req ens)
-  : (let c = TCspec #a #pre #post #req #ens pre' post' frame p0 p1 in
-     repr_steel_t a pre' post' (tree_req _ c) (tree_ens _ c))
+  : (let c = TCspec #a #pre #post #req #ens tcs in
+     repr_steel_t a tcs.tcs_pre tcs.tcs_post (tree_req _ c) (tree_ens _ c))
   = fun () ->
-    (**) steel_change_vequiv p0;
-    (**) steel_elim_vprop_of_list_append_f pre frame;
+    (**) steel_change_vequiv tcs.tcs_pre_eq;
+    (**) steel_elim_vprop_of_list_append_f pre tcs.tcs_frame;
     let x = f () in
-    (**) steel_intro_vprop_of_list_append_f (post x) frame;
-    (**) let sl1' = gget (vprop_of_list L.(post x @ frame)) in
-    (**) steel_change_vequiv (p1 x);
-    (**) let sl1'' = gget (vprop_of_list (post' x)) in
-    (**) assert (vpl_sels_f (post' x) sl1''
-    (**)      == extract_vars (p1 x) (vpl_sels_f L.(post x @ frame) sl1'));
-    (**) extract_vars_sym_l (p1 x) (vpl_sels_f L.(post x @ frame) sl1');
+    (**) steel_intro_vprop_of_list_append_f (post x) tcs.tcs_frame;
+    (**) let sl1' = gget (vprop_of_list L.(post x @ tcs.tcs_frame)) in
+    (**) steel_change_vequiv (tcs.tcs_post_eq x);
+    (**) let sl1'' = gget (vprop_of_list (tcs.tcs_post x)) in
+    (**) assert (vpl_sels_f (tcs.tcs_post x) sl1''
+    (**)      == extract_vars (tcs.tcs_post_eq x) (vpl_sels_f L.(post x @ tcs.tcs_frame) sl1'));
+    (**) extract_vars_sym_l (tcs.tcs_post_eq x) (vpl_sels_f L.(post x @ tcs.tcs_frame) sl1');
     Steel.Effect.Atomic.return x
 
 [@@ __repr_M__]
+let tree_of_steel_r
+      (#a : Type) (#pre : pre_t) (#post : post_t a) (#req : req_t pre) (#ens : ens_t pre a post)
+      ($f : repr_steel_t a pre post req ens)
+  : prog_tree a
+  = Tspec a pre post req ens
+
+[@@ __repr_M__]
 inline_for_extraction
-let repr_of_steel (#a : Type) (pre : pre_t) (post : post_t a) (req : req_t pre) (ens : ens_t pre a post)
-                  ($f : repr_steel_t a pre post req ens)
+let repr_of_steel_r
+      (#a : Type) (pre : pre_t) (post : post_t a) (req : req_t pre) (ens : ens_t pre a post)
+      ($f : repr_steel_t a pre post req ens)
+  : repr a
+  = {
+    repr_tree  = tree_of_steel_r f;
+    repr_steel = (fun pre'0 post'0 c ->
+                    let TCspec tcs = c in
+                    U.cast (repr_steel_t a pre'0 post'0 (tree_req _ c) (tree_ens _ c))
+                           (repr_of_steel_steel a pre post req ens tcs f))
+  }
+
+[@@ __repr_M__]
+let tree_of_steel
+      (#a : Type) (#pre : SE.pre_t) (#post : SE.post_t a) (#req : SE.req_t pre) (#ens : SE.ens_t pre a post)
+      ($f : unit_steel a pre post req ens)
+  : prog_tree a
+  = TspecS a pre post req ens
+
+[@@ __repr_M__]
+inline_for_extraction
+let repr_of_steel
+      (#a : Type) (pre : SE.pre_t) (post : SE.post_t a) (req : SE.req_t pre) (ens : SE.ens_t pre a post)
+      ($f : unit_steel a pre post req ens)
   : repr a
   = {
     repr_tree  = tree_of_steel f;
     repr_steel = (fun pre'0 post'0 c ->
-                    let (TCspec pre' post' frame  p0 p1) = c in
+                    let TCspecS tr tcs = c in
                     U.cast (repr_steel_t a pre'0 post'0 (tree_req _ c) (tree_ens _ c))
-                           (repr_of_steel_steel a pre post req ens pre' post' frame p0 p1 f))
+                           (repr_of_steel_steel a tr.r_pre tr.r_post tr.r_req tr.r_ens
+                                                tcs (repr_steel_of_steel tr f)))
   }
 
 
