experiment/Experiment.Steel.Repr.ST.fst
@@ -45,54 +45,117 @@ let equiv_Tbind_assoc_Tbind #a #b #c #pre #itm0 #itm1 #post f g h
 (***** Spec *)
 
 let norm_tree_spec () : T.Tac unit
-  = T.norm [delta_only [`%repr_ST_of_M; `%post_ST_of_M; `%bind; `%tree_req; `%tree_ens; `%const_post];
+  = T.norm [delta_only [`%repr_ST_of_M; `%repr_ST_of_M_Spec; `%post_ST_of_M; `%bind;
+                        `%tree_req; `%tree_ens; `%const_post; `%frame_post];
             delta_attr [`%U.__util_func__];
             delta_qualifier ["unfold"];
             zeta; iota; simplify]
 
-#push-options "--z3rlimit 15 --ifuel 1"
-let repr_ST_of_M__TCspec_ens
-      #a #pre #post (req : M.req_t pre) (ens : M.ens_t pre a post)
-      (pre' : M.pre_t) (post' : M.post_t a) (frame : vprop_list)
-      (p0 : vequiv pre' L.(pre @ frame)) (p1 : (x : a) -> vequiv (post x @ frame) (post' x))
-      (sl0' : sl_f pre') (res : a) (sl1' : sl_f (post' res))
+#push-options "--z3rlimit 15 --ifuel 0 --fuel 0"
+let repr_ST_of_M_Spec_ens
+      (#a : Type u#a) #pre #post (req : M.req_t pre) (ens : M.ens_t pre a post)
+      (tcs : tree_cond_Spec a pre post)
+      (sl0' : sl_f tcs.tcs_pre) (res : a) (sl1' : sl_f (tcs.tcs_post res))
 
   : Lemma (
-    (**) L.map_append Mkvprop'?.t pre frame;
-    (**) L.map_append Mkvprop'?.t (post res) frame;
+    (**) L.map_append Mkvprop'?.t pre tcs.tcs_frame;
+    (**) L.map_append Mkvprop'?.t (post res) tcs.tcs_frame;
 
-    (tree_ens (repr_ST_of_M _ (TCspec #a #pre #post #req #ens  pre' post' frame  p0 p1)) sl0' res sl1'
-    <==> (let sl0, frame0 = Fl.splitAt_ty (vprop_list_sels_t pre) (vprop_list_sels_t frame)
-                             (Fl.apply_pequiv (vequiv_sl p0) sl0') in
-        let sl1, frame1 = Fl.splitAt_ty (vprop_list_sels_t (post res)) (vprop_list_sels_t frame)
-                             (Fl.apply_pequiv (Perm.pequiv_sym (vequiv_sl (p1 res))) sl1') in
+    (tree_ens (repr_ST_of_M_Spec a pre post req ens tcs) sl0' res sl1'
+    <==> (let sl0, frame0 = Fl.splitAt_ty (vprop_list_sels_t pre) (vprop_list_sels_t tcs.tcs_frame)
+                             (Fl.apply_pequiv (vequiv_sl tcs.tcs_pre_eq) sl0') in
+        let sl1, frame1 = Fl.splitAt_ty (vprop_list_sels_t (post res)) (vprop_list_sels_t tcs.tcs_frame)
+                             (Fl.apply_pequiv (Perm.pequiv_sym (vequiv_sl (tcs.tcs_post_eq res))) sl1') in
         frame1 == frame0 /\ ens sl0 res sl1)))
   =
+    let frame = tcs.tcs_frame in
+    let p0 = tcs.tcs_pre_eq   in
+    let p1 = tcs.tcs_post_eq  in
     L.map_append Mkvprop'?.t pre frame;
     L.map_append Mkvprop'?.t (post res) frame;
     assert (
-      tree_ens (repr_ST_of_M _ (TCspec #a #pre #post #req #ens  pre' post' frame  p0 p1)) sl0' res sl1'
-    <==> (exists (sl1f : Fl.flist L.(vprop_list_sels_t (post res) @ vprop_list_sels_t frame)) .
-          let sl0, frame0 = Fl.splitAt_ty (vprop_list_sels_t pre) (vprop_list_sels_t frame)
-                               (Fl.apply_pequiv (vequiv_sl p0) sl0') in
-          let sl1, frame1 = Fl.splitAt_ty (vprop_list_sels_t (post res)) (vprop_list_sels_t frame) sl1f in
-          sl1' == Fl.apply_pequiv (vequiv_sl (p1 res)) sl1f /\
-          frame1 == frame0 /\ ens sl0 res sl1))
-      by T.(norm_tree_spec (); smt ());
+      tree_ens (repr_ST_of_M_Spec a pre post req ens tcs) sl0' res sl1'
+    ==
+     (exists (_ : U.unit' u#a) (sl0_0: Fl.flist (vprop_list_sels_t L.(pre @ frame))) .
+        eq2 #(Fl.flist (vprop_list_sels_t L.(pre @ frame)))
+            sl0_0 (Fl.apply_pequiv (vequiv_sl tcs.tcs_pre_eq) sl0') /\
+     (exists (x : a) (sl1_0 : Fl.flist L.(vprop_list_sels_t (post x) @ vprop_list_sels_t frame)) . (
+        (**) L.map_append Mkvprop'?.t (post x) tcs.tcs_frame; (
+        let sl0, frame0 = Fl.splitAt_ty (vprop_list_sels_t pre) (vprop_list_sels_t frame) sl0_0 in
+        let sl1, frame1 = Fl.splitAt_ty (vprop_list_sels_t (post x)) (vprop_list_sels_t frame) sl1_0 in
+        frame1 == frame0 /\ ens sl0 x sl1) /\
+     (exists (_u : U.unit' u#a) (sl1_1 : Fl.flist (vprop_list_sels_t (tcs.tcs_post x))) .
+        sl1_1 == Fl.apply_pequiv (vequiv_sl (tcs.tcs_post_eq x)) sl1_0 /\
+        (res == x /\ sl1' == sl1_1)))))
+    ) by T.(norm_tree_spec (); trefl ());
 
     introduce forall (sl1f : Fl.flist L.(vprop_list_sels_t (post res) @ vprop_list_sels_t frame)) .
         sl1' == Fl.apply_pequiv (vequiv_sl (p1 res)) sl1f <==>
         sl1f == Fl.apply_pequiv (Perm.pequiv_sym (vequiv_sl (p1 res))) sl1'
       with Fl.apply_pequiv_sym_eq_iff (vequiv_sl (p1 res)) sl1f sl1';
 
-    assert (tree_ens (repr_ST_of_M _ (TCspec #a #pre #post #req #ens  pre' post' frame  p0 p1)) sl0' res sl1'
-    <==> (let sl0, frame0 = Fl.splitAt_ty (vprop_list_sels_t pre) (vprop_list_sels_t frame)
-                             (Fl.apply_pequiv (vequiv_sl p0) sl0') in
-        let sl1, frame1 = Fl.splitAt_ty (vprop_list_sels_t (post res)) (vprop_list_sels_t frame)
-                             (Fl.apply_pequiv (Perm.pequiv_sym (vequiv_sl (p1 res))) sl1') in
+    assert (tree_ens (repr_ST_of_M_Spec a pre post req ens tcs) sl0' res sl1' <==> (
+        let sl1f = Fl.apply_pequiv (Perm.pequiv_sym (vequiv_sl (p1 res))) sl1' in
+        let sl0, frame0 = Fl.splitAt_ty (vprop_list_sels_t pre) (vprop_list_sels_t frame)
+                                        (Fl.apply_pequiv (vequiv_sl tcs.tcs_pre_eq) sl0') in
+        let sl1, frame1 = Fl.splitAt_ty (vprop_list_sels_t (post res)) (vprop_list_sels_t frame) sl1f in
         frame1 == frame0 /\ ens sl0 res sl1))
 #pop-options
 
+#push-options "--ifuel 0 --fuel 0"
+let repr_ST_of_M_req__Spec #a #pre #post req ens (tcs : tree_cond_Spec a pre post)
+                           (sl0 : sl_f tcs.tcs_pre)
+  : Lemma (M.spec_req tcs req sl0 <==> tree_req (repr_ST_of_M_Spec a pre post req ens tcs) sl0)
+  =
+    let frame = tcs.tcs_frame   in
+    let pre'  = tcs.tcs_pre     in
+    let p0    = tcs.tcs_pre_eq  in
+    L.map_append Mkvprop'?.t pre frame;
+
+    calc (<==>) {
+      M.spec_req tcs req sl0;
+    <==> { }
+      req (extract_vars_f tcs.tcs_pre pre tcs.tcs_frame tcs.tcs_pre_eq sl0)._1;
+    <==> { assert_norm (extract_vars_f pre' pre frame p0 sl0
+           == Fl.splitAt_ty (vprop_list_sels_t pre) (vprop_list_sels_t frame)
+                (Fl.apply_pequiv (vequiv_sl p0) sl0)) }
+      req (Fl.splitAt_ty (vprop_list_sels_t pre) (vprop_list_sels_t frame)
+                     (Fl.apply_pequiv (vequiv_sl p0) sl0))._1;
+    <==> { assert (tree_req (repr_ST_of_M_Spec a pre post req ens tcs) sl0
+            <==> req (Fl.splitAt_ty (vprop_list_sels_t pre) (vprop_list_sels_t frame)
+                     (Fl.apply_pequiv (vequiv_sl p0) sl0))._1)
+        by T.(norm_tree_spec (); smt ()) }
+      tree_req (repr_ST_of_M_Spec a pre post req ens tcs) sl0;
+    }
+
+let repr_ST_of_M_ens__Spec #a #pre #post req ens (tcs : tree_cond_Spec a pre post)
+                           (sl0 : sl_f tcs.tcs_pre) (x : a) (sl1 : sl_f (tcs.tcs_post x))
+  : Lemma (M.spec_ens tcs ens sl0 x sl1 <==> tree_ens (repr_ST_of_M_Spec a pre post req ens tcs) sl0 x sl1)
+  =
+    let frame = tcs.tcs_frame   in
+    let pre'  = tcs.tcs_pre     in
+    let post' = tcs.tcs_post    in
+    let p0    = tcs.tcs_pre_eq  in
+    let p1    = tcs.tcs_post_eq in
+    L.map_append Mkvprop'?.t pre frame;
+    L.map_append Mkvprop'?.t (post x) frame;
+    calc (<==>) {
+      M.spec_ens tcs ens sl0 x sl1;
+    <==> {_ by T.(apply_lemma (`U.iff_refl); trefl ()) }
+     (let fsl0, frame0 = extract_vars_f tcs.tcs_pre pre tcs.tcs_frame tcs.tcs_pre_eq sl0 in
+      let fsl1, frame1 = extract_vars_f (tcs.tcs_post x) (post x) tcs.tcs_frame
+                                        (Perm.pequiv_sym (tcs.tcs_post_eq x)) sl1 in
+       frame1 == frame0 /\ ens fsl0 x fsl1);
+    <==> { }
+     (let fsl0, frame0 = Fl.splitAt_ty (vprop_list_sels_t pre) (vprop_list_sels_t frame)
+                                         (Fl.apply_pequiv (vequiv_sl p0) sl0) in
+      let fsl1, frame1 = Fl.splitAt_ty (vprop_list_sels_t (post x)) (vprop_list_sels_t frame)
+                                         (Fl.apply_pequiv (Perm.pequiv_sym (vequiv_sl (p1 x))) sl1) in
+       frame1 == frame0 /\ ens fsl0 x fsl1);
+    <==> {repr_ST_of_M_Spec_ens req ens tcs sl0 x sl1}
+      tree_ens (repr_ST_of_M_Spec a pre post req ens tcs) sl0 x sl1;
+    }
+#pop-options
 
 #push-options "--z3rlimit 30 --ifuel 1"
 let rec repr_ST_of_M_req (#a : Type) (t : M.prog_tree a)
@@ -101,27 +164,11 @@ let rec repr_ST_of_M_req (#a : Type) (t : M.prog_tree a)
   : Lemma (ensures M.tree_req t c sl0 <==> tree_req (repr_ST_of_M t c) sl0)
           (decreases t)
   = match c as c returns squash (M.tree_req t c sl0 <==> tree_req (repr_ST_of_M t c) sl0) with
-  | TCspec #a #pre #post #req #ens  pre' post' frame  p0 p1 ->
-             L.map_append Mkvprop'?.t pre frame;
+  | TCspec #a #pre #post #req #ens  tcs ->
+             repr_ST_of_M_req__Spec req ens tcs sl0
 
-             calc (<==>) {
-               M.tree_req _ (TCspec #a #pre #post #req #ens  pre' post' frame  p0 p1) sl0;
-             <==> {_ by T.(apply_lemma (`U.iff_refl); trefl ()) }
-               req (extract_vars_f pre' pre frame p0 sl0)._1;
-             <==> { assert_norm (extract_vars_f pre' pre frame p0 sl0
-                    == Fl.splitAt_ty (vprop_list_sels_t pre) (vprop_list_sels_t frame)
-                         (Fl.apply_pequiv (vequiv_sl p0) sl0)) }
-               req (Fl.splitAt_ty (vprop_list_sels_t pre) (vprop_list_sels_t frame)
-                              (Fl.apply_pequiv (vequiv_sl p0) sl0))._1;
-             <==> { assert (tree_req (repr_ST_of_M _ (TCspec #a #pre #post #req #ens  pre' post' frame  p0 p1)) sl0
-                     <==> req (Fl.splitAt_ty (vprop_list_sels_t pre) (vprop_list_sels_t frame)
-                              (Fl.apply_pequiv (vequiv_sl p0) sl0))._1)
-                 by T.(norm_tree_spec (); smt ()) }
-               tree_req (repr_ST_of_M _ (TCspec #a #pre #post #req #ens  pre' post' frame  p0 p1)) sl0;
-             <==> { U.f_equal tree_req (repr_ST_of_M _ (TCspec #a #pre #post #req #ens  pre' post' frame  p0 p1))
-                                     (repr_ST_of_M _ c) }
-               tree_req (repr_ST_of_M _ c) sl0;
-             }
+  | TCspecS #a #pre #post #req #ens  tr tcs ->
+             repr_ST_of_M_req__Spec tr.r_req tr.r_ens tcs sl0
 
   | TCret #a #x #sl_hint  pre post  p ->
              U.f_equal tree_req (repr_ST_of_M _ (TCret #a #x #sl_hint pre post p))
@@ -183,29 +230,11 @@ and repr_ST_of_M_ens (#a : Type) (t : M.prog_tree a)
   : Lemma (ensures M.tree_ens t c sl0 res sl1 <==> tree_ens (repr_ST_of_M t c) sl0 res sl1)
           (decreases t)
   = match c as c returns squash (M.tree_ens t c sl0 res sl1 <==> tree_ens (repr_ST_of_M t c) sl0 res sl1) with
-    | TCspec #a #pre #post #req #ens  pre' post' frame  p0 p1 ->
-             L.map_append Mkvprop'?.t pre frame;
-             L.map_append Mkvprop'?.t (post res) frame;
+    | TCspec #a #pre #post #req #ens  tcs ->
+             repr_ST_of_M_ens__Spec req ens tcs sl0 res sl1
 
-             calc (<==>) {
-               M.tree_ens _ (TCspec #a #pre #post #req #ens  pre' post' frame  p0 p1) sl0 res sl1;
-             <==> {_ by T.(apply_lemma (`U.iff_refl); trefl ()) }
-              (let fsl0, frame0 = extract_vars_f pre' pre frame p0 sl0 in
-               let fsl1, frame1 = extract_vars_f (post' res) (post res) frame
-                                                 (Perm.pequiv_sym (p1 res)) sl1 in
-                frame1 == frame0 /\ ens fsl0 res fsl1);
-             <==> { }
-              (let fsl0, frame0 = Fl.splitAt_ty (vprop_list_sels_t pre) (vprop_list_sels_t frame)
-                                                  (Fl.apply_pequiv (vequiv_sl p0) sl0) in
-               let fsl1, frame1 = Fl.splitAt_ty (vprop_list_sels_t (post res)) (vprop_list_sels_t frame)
-                                                  (Fl.apply_pequiv (Perm.pequiv_sym (vequiv_sl (p1 res))) sl1) in
-                frame1 == frame0 /\ ens fsl0 res fsl1);
-             <==> {repr_ST_of_M__TCspec_ens req ens pre' post' frame p0 p1 sl0 res sl1}
-               tree_ens (repr_ST_of_M _ (TCspec #a #pre #post #req #ens  pre' post' frame p0 p1)) sl0 res sl1;
-             <==> {U.f_equal tree_ens (repr_ST_of_M _ (TCspec #a #pre #post #req #ens  pre' post' frame  p0 p1))
-                                    (repr_ST_of_M _ c)}
-               tree_ens (repr_ST_of_M _ c) sl0 res sl1;
-             }
+  | TCspecS #a #pre #post #req #ens  tr tcs ->
+             repr_ST_of_M_ens__Spec tr.r_req tr.r_ens tcs sl0 res sl1
 
   | TCret #a #x #sl_hint  pre post  p ->
              calc (<==>) {
@@ -272,7 +301,8 @@ and repr_ST_of_M_ens (#a : Type) (t : M.prog_tree a)
 (***** Shape *)
 
 let repr_ST_of_M_shape__norm : list norm_step =
-  [delta_only [`%prog_has_shape'; `%repr_ST_of_M; `%shape_ST_of_M; `%bind];
+  [delta_only [`%prog_has_shape'; `%repr_ST_of_M; `%repr_ST_of_M_Spec; `%shape_ST_of_M; `%bind];
+   delta_qualifier ["unfold"];
    iota; zeta]
 
 #push-options "--ifuel 1"
@@ -283,22 +313,27 @@ let rec repr_ST_of_M_shape
    : Lemma (requires M.tree_cond_has_shape c s)
            (ensures  prog_has_shape (repr_ST_of_M t c) (shape_ST_of_M s))
    = match c with
-   | TCspec #a #pre #post #req #ens pre1 post1 frame p0 p1 ->
+   | TCspec #a #pre #post #req #ens tcs ->
             let M.Sspec pre_n post_n frame_n p0' p1' = s in
-            assert (prog_has_shape' (repr_ST_of_M t (TCspec #a #pre #post #req #ens pre1 post1 frame p0 p1))
+            assert (prog_has_shape' (repr_ST_of_M t (TCspec #a #pre #post #req #ens tcs))
                                     (shape_ST_of_M (M.Sspec pre_n post_n frame_n p0' p1')))
                 by T.(norm repr_ST_of_M_shape__norm; smt ())
-  | TCret #a #x #sl_hint  pre post p ->
+   | TCspecS #a #pre #post #req #ens tr tcs ->
+            let M.Sspec pre_n post_n frame_n p0' p1' = s in
+            assert (prog_has_shape' (repr_ST_of_M t (TCspecS #a #pre #post #req #ens tr tcs))
+                                    (shape_ST_of_M (M.Sspec pre_n post_n frame_n p0' p1')))
+                by T.(norm repr_ST_of_M_shape__norm; smt ())
+   | TCret #a #x #sl_hint  pre post p ->
             let M.Sret n p' = s in
             assert (prog_has_shape' (repr_ST_of_M t (TCret #a #x #sl_hint pre post p))
                                     (shape_ST_of_M (M.Sret n p')))
                 by T.(norm repr_ST_of_M_shape__norm; smt ())
-  | TCbind #a #b #f #g _ _ _ cf cg ->
+   | TCbind #a #b #f #g _ _ _ cf cg ->
             let M.Sbind _ _ _ s_f s_g = s in
             repr_ST_of_M_shape f cf s_f;
             introduce forall (x : a) . prog_has_shape (repr_ST_of_M (g x) (cg x)) (shape_ST_of_M s_g)
               with repr_ST_of_M_shape (g x) (cg x) s_g
-  | TCbindP #a #b #_ #_ #g _ _ cg ->
+   | TCbindP #a #b #_ #_ #g _ _ cg ->
             let M.SbindP _ _ s_g = s in
             introduce forall (x : a) . prog_has_shape (repr_ST_of_M (g x) (cg x)) (shape_ST_of_M s_g)
               with repr_ST_of_M_shape (g x) (cg x) s_g
