experiment/Experiment.Steel.Repr.ST.fsti
@@ -129,7 +129,7 @@ and tree_ens (#a : Type) (#pre : pre_t) (#post : post_t a) (t : prog_tree a pre 
   = match t with
   | Tequiv _ post p ->
              (fun sl0 _ sl1 ->
-               sl1 == Fl.apply_pequiv p sl0)
+               eq2 #(Fl.flist post) sl1 (Fl.apply_pequiv p sl0))
   | Tframe a  pre post frame f ->
              (fun sl0 x sl1 ->
                let sl0', frame0 = Fl.splitAt_ty pre      frame sl0 in
@@ -297,21 +297,32 @@ let mk_prog_shape (#a : Type) (#pre : pre_t) (#post : post_t a) (t : prog_tree a
 let post_ST_of_M (#a : Type) (post : M.post_t a) : post_t a
   = fun (x : a) -> vprop_list_sels_t (post x)
 
+let repr_ST_of_M_Spec
+      (a : Type) (pre : M.pre_t) (post : M.post_t a) (req : M.req_t pre) (ens : M.ens_t pre a post)
+      (tcs : tree_cond_Spec a pre post)
+  : prog_tree a (vprop_list_sels_t tcs.tcs_pre) (post_ST_of_M tcs.tcs_post)
+  =
+    Tequiv (vprop_list_sels_t tcs.tcs_pre)
+           (vprop_list_sels_t L.(pre @ tcs.tcs_frame))
+           (vequiv_sl tcs.tcs_pre_eq);;
+    (**) L.map_append Mkvprop'?.t pre tcs.tcs_frame;
+    x <-- Tframe a (vprop_list_sels_t pre) (post_ST_of_M post) (vprop_list_sels_t tcs.tcs_frame)
+        (Tspec a (vprop_list_sels_t pre) (post_ST_of_M post) req ens);
+    (**) L.map_append Mkvprop'?.t (post x) tcs.tcs_frame;
+    Tequiv (vprop_list_sels_t L.(post x @ tcs.tcs_frame))
+           (vprop_list_sels_t (tcs.tcs_post x))
+           (vequiv_sl (tcs.tcs_post_eq x));;
+    Tret _ x (post_ST_of_M tcs.tcs_post)
+
 let rec repr_ST_of_M (#a : Type) (t : M.prog_tree u#a a)
                      (#pre0 : M.pre_t) (#post0 : M.post_t a) (c : M.tree_cond t pre0 post0)
   : Tot (prog_tree a (vprop_list_sels_t pre0) (post_ST_of_M post0))
         (decreases t)
   = match c with
-  | TCspec #a #pre #post #req #ens  pre' post' frame  p0 p1 ->
-             Tequiv (vprop_list_sels_t pre') (vprop_list_sels_t L.(pre@frame)) (vequiv_sl p0);;
-             (**) L.map_append Mkvprop'?.t pre frame;
-             x <-- Tframe a (vprop_list_sels_t pre) (post_ST_of_M post) (vprop_list_sels_t frame)
-                 (Tspec a (vprop_list_sels_t pre) (post_ST_of_M post) req ens);
-             (**) L.map_append Mkvprop'?.t (post x) frame;
-             Tequiv (vprop_list_sels_t L.(post x @ frame))
-                    (vprop_list_sels_t (post' x))
-                    (vequiv_sl (p1 x));;
-             Tret _ x (post_ST_of_M post')
+  | TCspec #a #pre #post #req #ens  tcs ->
+             repr_ST_of_M_Spec a pre post req ens tcs
+  | TCspecS #a tr tcs ->
+             repr_ST_of_M_Spec a tr.r_pre tr.r_post tr.r_req tr.r_ens tcs
   | TCret #a #x #_  pre post  p ->
              Tequiv (vprop_list_sels_t pre) (vprop_list_sels_t (post x)) (vequiv_sl p);;
              Tret _ x (post_ST_of_M post)
