experiment/Experiment.Steel.fsti
@@ -84,6 +84,7 @@ let prog_M_to_Fun_extract_wp
       (fun sl0 -> wp sl0; Fun.tree_wp_sound (prog_M_to_Fun t c sl0) (fun res -> ens sl0 res.val_v res.sel_v))
 
 
+(**** normalisation steps *)
 
 let __normal_M : list norm_step = [
   delta_only [`%M.vprop_list_sels_t;     `%M.Mkrepr?.repr_tree;
@@ -97,7 +98,7 @@ let __normal_M : list norm_step = [
 ]
 
 let __normal_ST : list norm_step = [
-  delta_only [`%ST.repr_ST_of_M; `%ST.bind; `%ST.post_ST_of_M;
+  delta_only [`%ST.repr_ST_of_M; `%ST.repr_ST_of_M_Spec; `%ST.bind; `%ST.post_ST_of_M;
               `%M.vprop_list_sels_t; `%L.map; `%SE.Mkvprop'?.t;
               `%ST.const_post; `%ST.frame_post; `%L.op_At; `%L.append;
               `%ST.flatten_prog; `%ST.flatten_prog_aux; `%ST.flatten_prog_k_id;
@@ -106,7 +107,7 @@ let __normal_ST : list norm_step = [
               `%M.Mkprog_cond?.pc_tree;  `%M.Mkprog_cond?.pc_post_len; `%M.Mkprog_cond?.pc_shape;
               `%Perm.perm_f_to_list; `%Ll.initi; `%Perm.id_n; `%Perm.mk_perm_f];
   delta_qualifier ["unfold"];
-  delta_attr [`%SE.__steel_reduce__];
+  delta_attr [`%__tac_helper__; `%SE.__steel_reduce__];
   iota; zeta; primops
 ]
 
@@ -182,23 +183,6 @@ let __normal_vprop_list : list norm_step = [
   iota; zeta; primops
 ]
 
-/// Steps for normalizing [M.flatten_vprop v].
-let __normal_flatten_vprop : list norm_step = [
-  delta_only [`%M.flatten_vprop; `%M.flatten_vprop_aux];
-  delta_attr [`%SE.__reduce__];
-  delta_qualifier ["unfold"];
-  iota; zeta; primops
-]
-
-/// Steps for the normalisation of Steel's requires and ensures clauses.
-/// We need [__steel_reduce__] in order to unfold the selector functions
-/// (for instance [Steel.Reference.sel])
-let __normal_Steel_logical_spec : list norm_step = [
-  delta_only [`%SE.VUnit?._0];
-  delta_attr [`%SE.__reduce__; `%SE.__steel_reduce__];
-  delta_qualifier ["unfold"];
-  iota; zeta; primops
-]
 
 (***** Calling a [M.repr_steel_t] from a Steel program *)
 
@@ -294,213 +278,6 @@ let solve_by_wp () : Tac unit
 
 (***** Extracting a [M.unit_steel] from a [M.repr] *)
 
-(*// This fail, seemingly because of the expansion of the memories when checking the post
-[@@ handle_smt_goals ]
-let tac () = dump "SMT query"
-let steel_of_repr
-      (#a : Type) (#pre : SE.pre_t) (#post : SE.post_t a) (#req : SE.req_t pre) (#ens : SE.ens_t pre a post)
-      (f : M.unit_steel a pre post req ens)
-  : SE.Steel a pre post req ens
-  = f ()*)
-
-[@@ __tac_helper__]
-noeq
-type to_repr_t (a : Type) (pre : SE.pre_t) (post : SE.post_t a) (req : SE.req_t pre) (ens : SE.ens_t pre a post)
-= {
-  r_pre  : M.pre_t;
-  r_post : M.post_t a;
-  r_req  : M.req_t r_pre;
-  r_ens  : M.ens_t r_pre a r_post;
-  r_pre_eq  : unit -> Lemma (pre `SE.equiv` M.vprop_of_list r_pre);
-  r_post_eq : (x : a) -> Lemma (post x `SE.equiv` M.vprop_of_list (r_post x));
-  r_req_eq  : (h0 : SE.rmem pre) -> Lemma (req h0 ==
-                  r_req (M.sel r_pre (
-                          r_pre_eq ();
-                          SE.equiv_can_be_split pre (M.vprop_of_list r_pre);
-                          SE.focus_rmem h0 (M.vprop_of_list r_pre))));
-  r_ens_eq  : (h0 : SE.rmem pre) -> (x : a) -> (h1 : SE.rmem (post x)) -> Lemma (ens h0 x h1 ==
-                  r_ens (M.sel r_pre (
-                          r_pre_eq ();
-                          SE.equiv_can_be_split pre (M.vprop_of_list r_pre);
-                          SE.focus_rmem h0 (M.vprop_of_list r_pre)))
-                        x
-                        (M.sel (r_post x) (
-                          r_post_eq x;
-                          SE.equiv_can_be_split (post x) (M.vprop_of_list (r_post x));
-                          SE.focus_rmem h1 (M.vprop_of_list (r_post x)))))
-}
-
-inline_for_extraction
-val steel_of_repr
-      (#a : Type) (#pre : SE.pre_t) (#post : SE.post_t a) (#req : SE.req_t pre) (#ens : SE.ens_t pre a post)
-      (tr : to_repr_t a pre post req ens)
-      (f : M.repr_steel_t a tr.r_pre tr.r_post tr.r_req tr.r_ens)
-  : M.unit_steel a pre post req ens
-
-val __build_to_repr_t_lem
-      (p : SE.vprop) (r_p : M.vprop_list {p `SE.equiv` M.vprop_of_list r_p}) (h : SE.rmem p)
-      (v : SE.vprop{SE.can_be_split p v}) (_ : squash (SE.VUnit? v))
-      (i : CSl.elem_index (SE.VUnit?._0 v) r_p)
-      (i' : int) (_ : squash (i' == i))
-  : squash (h v ==
-        M.sel r_p (SE.equiv_can_be_split p (M.vprop_of_list r_p);
-                   SE.focus_rmem h (M.vprop_of_list r_p)) i)
-
-[@@ __tac_helper__]
-let __build_to_repr_t
-      (#a : Type) (#pre : SE.pre_t) (#post : SE.post_t a) (#req : SE.req_t pre) (#ens : SE.ens_t pre a post)
-
-      (e_pre  : M.vprop_with_emp pre) (r_pre  : M.pre_t)
-      (pre_eq  : squash (r_pre == M.flatten_vprop e_pre))
-
-      (e_post : (x : a) -> M.vprop_with_emp (post x)) (r_post : M.post_t a)
-      (post_eq : (x : a) -> squash (r_post x == M.flatten_vprop (e_post x)))
-
-      (#r_req  : M.req_t r_pre)
-      (r_req_eq  : (h0 : SE.rmem pre) -> (sl0 : M.sl_f r_pre) ->
-                   (sl0_eq : ((v : SE.vprop{SE.can_be_split pre v}) -> squash (SE.VUnit? v) ->
-                             (i : CSl.elem_index (SE.VUnit?._0 v) r_pre) ->
-                             // This indirection is needed so that [apply_raw] presents a goal for [i]
-                             (i' : int) -> (_ : squash (i' == i)) ->
-                             squash (h0 v == sl0 i'))) ->
-                    r_req sl0 == req h0)
-
-      (#r_ens  : M.ens_t r_pre a r_post)
-      (r_ens_eq  : (h0 : SE.rmem pre) -> (sl0 : M.sl_f r_pre) ->
-                   (x : a) ->
-                   (h1 : SE.rmem (post x)) -> (sl1 : M.sl_f (r_post x)) ->
-                   (sl0_eq : ((v : SE.vprop{SE.can_be_split pre v}) -> squash (SE.VUnit? v) ->
-                             (i : CSl.elem_index (SE.VUnit?._0 v) r_pre) ->
-                             (i' : int) -> (_ : squash (i' == i)) ->
-                             squash (h0 v == sl0 i'))) ->
-                   (sl1_eq : ((v : SE.vprop{SE.can_be_split (post x) v}) -> squash (SE.VUnit? v) ->
-                             (i : CSl.elem_index (SE.VUnit?._0 v) (r_post x)) ->
-                             (i' : int) -> (_ : squash (i' == i)) ->
-                             squash (h1 v == sl1 i'))) ->
-                   r_ens sl0 x sl1 == ens h0 x h1)
-
-  : to_repr_t a pre post req ens
-  = 
-    let r_pre_eq () : Lemma (pre `SE.equiv` M.vprop_of_list r_pre)
-      = pre_eq;
-        M.vprop_equiv_flat pre e_pre;
-        SE.equiv_sym (M.vprop_of_list r_pre) pre                in
-    let r_post_eq (x : a) : Lemma (post x `SE.equiv` M.vprop_of_list (r_post x))
-      = post_eq x;
-        M.vprop_equiv_flat (post x) (e_post x);
-        SE.equiv_sym (M.vprop_of_list (r_post x)) (post x)
-    in
-    {
-    r_pre; r_post; r_req; r_ens;
-    r_pre_eq; r_post_eq;
-    r_req_eq  = (fun (h0 : SE.rmem pre) ->
-                   r_pre_eq ();
-                   SE.equiv_can_be_split pre (M.vprop_of_list r_pre);
-                   let h0_r = SE.focus_rmem h0 (M.vprop_of_list r_pre) in
-                   r_req_eq h0 (M.sel r_pre h0_r)
-                            (__build_to_repr_t_lem pre r_pre h0));
-    r_ens_eq  = (fun (h0 : SE.rmem pre) (x : a) (h1 : SE.rmem (post x)) ->
-                   r_pre_eq ();
-                   SE.equiv_can_be_split pre (M.vprop_of_list r_pre);
-                   let h0_r = SE.focus_rmem h0 (M.vprop_of_list r_pre) in
-                   r_post_eq x;
-                   SE.equiv_can_be_split (post x) (M.vprop_of_list (r_post x));
-                   let h1_r = SE.focus_rmem h1 (M.vprop_of_list (r_post x)) in
-                   r_ens_eq h0 (M.sel r_pre h0_r) x h1 (M.sel (r_post x) h1_r)
-                            (__build_to_repr_t_lem pre r_pre h0)
-                            (__build_to_repr_t_lem (post x) (r_post x) h1))
-  }
-
-(**) private val __begin_tacs : unit
-
-let filter_rmem_apply (#p : SE.vprop) (h : SE.rmem p) (v : SE.vprop{SE.can_be_split p v})
-  #sl (_ : squash (h v == sl))
-  : squash (h v == sl)
-  = ()
-
-/// Given a term [squash (lhs == rhs)], this tactics returns [Some (h, v)] if [lhs] is [h v]
-/// UNUSED: using v generates a SMT goal [SE.can_be_split]
-let match_rmem_apply (t : term) : Tac (option (term & term))
-  = match inspect t with
-    | Tv_App _squash (eq, Q_Explicit) ->
-      let _, ts = collect_app eq in
-      let n_args = L.length ts in
-      if n_args <> 3 then fail ("unexpected shape1:"^string_of_int n_args)
-      else let lhs = (L.index ts 1)._1 in
-     (match inspect lhs with
-      | Tv_App h (v, Q_Explicit) -> Some (h, v)
-      | _ -> None)
-    | _ -> fail "unexpected shape0"
-
-/// Solves a goal [to_repr_t a pre post req ens]
-let build_to_repr_t () : Tac unit
-  =
-    let u_r_pre  = fresh_uvar None in
-    let u_r_post = fresh_uvar None in
-    let u_r_req  = fresh_uvar None in
-    let u_r_ens  = fresh_uvar None in
-    apply_raw (`__build_to_repr_t);
-
-    (* [r_pre] *)
-    CSl.build_vprop_with_emp ();
-    exact u_r_pre;
-    norm __normal_flatten_vprop;
-    trefl ();
-
-    (* [r_post] *)
-    let _ = intro () in
-      CSl.build_vprop_with_emp ();
-    exact u_r_post;
-    let _ = intro () in
-      norm __normal_flatten_vprop;
-      trefl ();
-
-    // apply the rewriting hypothesis [eq_lem] to solve a goal [squash (h v == sl ?i)]
-    let apply_rew eq_lem =
-      apply_raw eq_lem;
-      // [VUnit?]
-      norm [delta_only [`%SE.VUnit?]; iota];
-      trivial ();
-      // [elem_index]
-      norm __normal_Steel_logical_spec;
-      CSl.build_elem_index ();
-      // [i' <- i]
-      norm [delta_attr [`%CSl.__cond_solver__; `%__tac_helper__]];
-      trefl ()
-    in
-
-    (* [r_req] *)
-    exact u_r_req;
-    let h0 = intro () in let sl0 = intro () in let eq0 = intro () in
-      // This normalisation has to be done after introducing [eq0], otherwise its application fails,
-      // seemingly because of the normalisation of [t_of].
-      norm __normal_Steel_logical_spec;
-      pointwise begin fun () ->
-        match catch (fun () -> apply_raw (`filter_rmem_apply (`#h0))) with
-        | Inr () -> // For some reason, this can only be applied on the goal produced by [filter_rmem_apply]
-                   apply_rew eq0
-        | Inl _  -> trefl ()
-      end;
-      trefl ();
-
-    (* [r_ens] *)
-    exact u_r_ens;
-    let h0  = intro () in let sl0 = intro () in
-    let x   = intro () in
-    let h1  = intro () in let sl1 = intro () in
-    let eq0 = intro () in let eq1 = intro () in
-      norm __normal_Steel_logical_spec;
-      pointwise begin fun () ->
-        match catch (fun () -> apply_raw (`filter_rmem_apply (`#h0))) with
-        | Inr () -> apply_rew eq0
-        | Inl _ ->
-        match catch (fun () -> apply_raw (`filter_rmem_apply (`#h1))) with
-        | Inr () -> apply_rew eq1
-        | Inl _  -> trefl ()
-      end;
-      trefl ()
-
-
 /// Similarly to [extract], [t] is only mentioned so that it can be retrieved by the tactic
 type __to_steel_goal
       (a : Type) (pre : SE.pre_t) (post : SE.post_t a) (req : SE.req_t pre) (ens : SE.ens_t pre a post)
@@ -512,10 +289,10 @@ inline_for_extraction
 let __build_to_steel
       (#a : Type) (#pre : SE.pre_t) (#post : SE.post_t a) (#req : SE.req_t pre) (#ens : SE.ens_t pre a post)
       (#t : M.repr a)
-      (goal_tr : to_repr_t a pre post req ens)
+      (goal_tr : M.to_repr_t a pre post req ens)
       (goal_f  : extract a goal_tr.r_pre goal_tr.r_post goal_tr.r_req goal_tr.r_ens t)
   : __to_steel_goal a pre post req ens t
-  = steel_of_repr goal_tr goal_f
+  = M.steel_of_repr goal_tr goal_f
 
 /// Solves a goal [__to_steel_goal]
 // FIXME: this tactic get stuck if this file is lax-checked
@@ -529,7 +306,7 @@ let build_to_steel () : Tac unit
     // [__lax_made] introduced for the specifications.
     let t = timer_start "specs     " in
     apply_raw (`__build_to_steel);
-    build_to_repr_t ();
+    CSl.build_to_repr_t ();
     timer_stop t;
 
     // [extract]
@@ -545,5 +322,3 @@ let to_steel
       (g : __to_steel_goal a pre post req ens t)
   : M.unit_steel a pre post req ens
   = g
-
-(**) private val __end_tacs : unit
