experiment/Experiment.Steel.CondSolver.Test.fst
@@ -45,13 +45,28 @@ let test_TCspec_u (v0 v1 : vprop') : squash True =
         let _ =
           build (`(M.tree_cond (specT int [(`@v0)] (fun _ -> [(`@v1)]))
                                [(`@v0)] (`#post')))
-          (fun () -> norm_test (); build_TCspec false)
+          (fun () -> norm_test (); build_TCspec false false)
         in ())
 
 let test_TCspec_p (v0 v1 v2 : vprop') (vx : int -> vprop')
   : M.tree_cond (specT int [v0; v1] (fun x -> [v0; vx x]))
                 ([v0; v1; v2]) (fun x -> [v2; vx x; v0])
-  = _ by (norm_test (); let _ = build_TCspec true in ())
+  = _ by (norm_test (); let _ = build_TCspec false true in ())
+
+
+let test_TCspecS_u (v0 v1 : vprop') : squash True =
+  _ by (let post' = fresh_uvar (Some (`(M.post_t int))) in
+        let _ =
+          build (`(M.tree_cond (M.TspecS int (VUnit (`@v0)) (fun _ -> VUnit (`@v1)) (fun _ -> True) (fun _ _ _ -> True))
+                               [(`@v0)] (`#post')))
+          (fun () -> norm_test (); build_TCspec true false)
+        in ())
+
+let test_TCspecS_p (v0 v1 v2 : vprop') (vx : int -> vprop')
+  : M.tree_cond (M.TspecS int (VUnit v0 `star` VUnit v1) (fun x -> VUnit v0 `star` VUnit (vx x))
+                            (fun _ -> True) (fun _ _ _ -> True))
+                ([v0; v1; v2]) (fun x -> [v2; vx x; v0])
+  = _ by (norm_test (); let _ = build_TCspec true true in ())
 
 
 let test_TCret_u (v0 v1 : vprop') : squash True =
@@ -77,12 +92,12 @@ let test_TCbind_u (v0 v1 : vprop') (vx0 : int -> vprop') : squash True =
           (fun () ->
             norm_test ();
             apply (`M.TCbind);
-            let _ = build_TCspec false in
+            let _ = build_TCspec false false in
             let x = intro () in
             norm_cond_sol ();
             let post1 = fresh_uvar None in
             apply_raw (`(__defer_post_unification (`#post1)));
-            let _ = build_TCspec false in
+            let _ = build_TCspec false false in
             norm_cond_sol (); trefl ()
           )
         in ())
@@ -95,10 +110,10 @@ let test_TCbind_p (v0 v1 : vprop') (vx0 vx1 : int -> vprop')
   = _ by (
     norm_test ();
     apply (`M.TCbind);
-    let _ = build_TCspec false in
+    let _ = build_TCspec false false in
     let x = intro () in
     norm_cond_sol ();
-    let _ = build_TCspec true in
+    let _ = build_TCspec false true in
     ()
   )
 
@@ -116,7 +131,7 @@ let test_TCbindP_u (v0 v1 : vprop') (vx0 : int -> vprop') (wp : pure_wp int) (f 
             let x = intro () in
             let post1 = fresh_uvar None in
             apply_raw (`(__defer_post_unification (`#post1)));
-            let _ = build_TCspec false in
+            let _ = build_TCspec false false in
             norm_cond_sol (); trefl ()
           )
         in ())
@@ -130,7 +145,7 @@ let test_TCbindP_p (v0 v1 : vprop') (vx0 : int -> vprop') (wp : pure_wp int) (f 
     norm_test ();
     apply (`M.TCbindP);
     let x = intro () in
-    let _ = build_TCspec true in ()
+    let _ = build_TCspec false true in ()
   )
 
 
@@ -227,7 +242,7 @@ let test_steel__ret_f (v : int -> vprop) (x : int) (f : int -> int)
   : SteelT int (v (f x)) (fun y -> v y)
   = Steel.Effect.Atomic.return (f x)
 
-(* TODO : allow ghost post
+(* TODO : mark vprop' as erasable
 let test_build_tree_cond__ret_ghost (r : ref int)
   : M.tree_cond
         (M.Tret (Ghost.erased (ref int)) (Ghost.hide r) (fun _ -> []))
